Reflexive-transitive closure for well-founded relations (#7)
Computable reflexive-transitive closure of well-founded functions

relations.v
@@ -1,29 +1,167 @@
 From Coq Require Import Lia.
-From Coq Require Import Relations.
-From mathcomp Require Import ssreflect ssrbool eqtype ssrnat ssrfun fintype.
+
+From Coq Require Import Relations Program.Basics.
+From mathcomp Require Import ssreflect ssrbool eqtype ssrfun seq order.
 From Equations Require Import Equations.
-From event_struct Require Import utilities.
+From event_struct Require Import utilities wftype.
 
 Set Implicit Arguments.
-Unset Strict Implicit.
+(* Unset Strict Implicit. *)
 Unset Printing Implicit Defensive.
+Set Equations Transparent.
+
+Import Order.LTheory.
+Local Open Scope order_scope.
 
 Section well_founded.
 
-Variable irel : rel nat.
+Definition sfrel {T : eqType} (f : T -> seq T) : rel T :=
+  [rel a b | b \in f a].
 
-Definition rt_cl : rel nat. Admitted.
+Definition filter_neq {T : eqType} (f : T -> seq T) : T -> seq T :=
+  fun n => filter^~ (f n) (fun x => x != n).
 
-Lemma irel_rt_cl : subrel irel rt_cl. Admitted.
+Notation "f '\eq'" := (filter_neq f) (at level 5, format "f '\eq'").
 
-Lemma rt_cl_refl: reflexive rt_cl.
-Proof. Admitted.
+Context {T : wfType}.
 
-Lemma rt_cl_trans: transitive rt_cl.
-Proof. Admitted.
+Variable (f : T -> seq T).
 
-Lemma closureP e1 e2: 
-  reflect (clos_refl_trans_n1 _ irel e1 e2) (rt_cl e1 e2).
-Proof. Admitted.
+Hypothesis descend : forall x n, x \in f n -> x <= n.
+
+Lemma filter_lt n k : k \in f\eq n -> k < n.
+Proof. by rewrite mem_filter lt_neqAle => /andP[] -> /descend ->. Qed.
+
+Lemma rel_sublt a b : (sfrel f\eq) a b -> b < a.
+Proof. rewrite/sfrel /=. exact: filter_lt. Qed.
+
+(* Computation of the strict upward set of a given element
+ * w.r.t relation R derived from function `f`,
+ * i.e. s_up_set(x) = { y | x R y } 
+ *)
+Equations(noind) s_up_set (n : T) : seq T by wf n (<%O : rel T) :=
+  s_up_set n := 
+    let ys := f\eq n in 
+    let ps := flatten (map^~ ys (fun x => 
+      if x \in ys =P true is ReflectT pf then
+        s_up_set x
+      else 
+        [::]
+    )) in
+    ys ++ ps.
+Next Obligation. exact: filter_lt. Qed.
+
+Definition t_closure (a b : T) : bool := b \in s_up_set a.
+
+Lemma ext_s_up_set (x : T) (g h : forall y : T, y < x -> seq T) :
+  (forall (y : T) (p : y < x), g y p = h y p) ->
+    s_up_set_functional x g = s_up_set_functional x h.
+Proof.
+  move=> H. rewrite /s_up_set_functional. apply/eqP.
+  rewrite eqseq_cat //=. apply/andP. split=> //=. apply/eqP.
+  congr flatten. apply/eq_in_map. move=> y /filter_lt. case: eqP=> //=.
+Qed.
+
+Lemma t_closure_lt a b : t_closure a b -> b < a.
+Proof.
+  rewrite /t_closure.
+  move: a b. apply: wf_ind => a IH b.
+  rewrite /s_up_set /Subterm.FixWf Fix_eq; last by apply: ext_s_up_set.
+  rewrite {1}/s_up_set_functional mem_cat => /orP [/filter_lt //|].
+  case/flatten_mapP=> x /filter_lt xinf.
+  case: eqP => //. move=> /filter_lt /IH /apply ax. 
+  by apply: lt_trans; first apply: ax.
+Qed.
+
+Lemma clos_trans_lt a b : clos_trans_n1 T (sfrel f\eq) a b -> b < a.
+Proof.
+  rewrite/sfrel /=.
+  elim=> [x /filter_lt // | x y xfy acx ax].
+  apply: lt_trans; last by apply: ax.
+  exact: filter_lt.
+Qed. 
+
+(* Transitive closure reflection lemma *)
+Lemma t_closureP a b : 
+  reflect (clos_trans_1n T (sfrel f\eq) a b) (t_closure a b).
+Proof.
+  rewrite /t_closure.
+  move: a b. apply: wf_ind=> a IH b.
+  apply /(iffP idP).
+  { rewrite /s_up_set /Subterm.FixWf Fix_eq; last by apply: ext_s_up_set.
+    rewrite {1}/s_up_set_functional mem_cat => /orP [].
+    { by constructor. }
+    case/flatten_mapP=> x xinf. case: eqP=> //=.
+    move=> /filter_lt /IH /apply H.
+    apply: Relation_Operators.t1n_trans; last exact H.
+    exact xinf. }
+  move=> ctab. move: ctab IH. case.
+  { rewrite /sfrel /= => c afc IH.
+    rewrite /s_up_set /Subterm.FixWf Fix_eq; last by apply: ext_s_up_set.
+    by rewrite {1}/s_up_set_functional mem_cat afc. }
+  move=> c d. rewrite /sfrel /= => cfd ctac IHd.
+  rewrite /s_up_set /Subterm.FixWf Fix_eq; last by apply: ext_s_up_set.
+  rewrite {1}/s_up_set_functional mem_cat. apply/orP.
+  right. apply/flatten_mapP. exists c=> //=. case: eqP=> //=.
+  move=> _. apply/IHd=> //=. exact: filter_lt.
+Qed.
+
+
+(* Computation of the (non-strict) upward set of a given element
+ * w.r.t relation R derived from function `f`,
+ * i.e. up_set(x) = { y | x = y \/ x R y } 
+ *)
+Definition up_set a := a :: s_up_set a.
+
+Definition rt_closure a b := b \in up_set a. 
+
+Lemma rt_closure_refl a : rt_closure a a.
+Proof. rewrite /rt_closure /up_set. exact: mem_head. Qed.
+
+Lemma rt_closure_trans a b c :
+  rt_closure a b -> rt_closure b c -> rt_closure a c.
+Proof.
+  rewrite /rt_closure.
+  rewrite !in_cons => /orP [/eqP -> //|].
+  move=> ba /orP [/eqP -> //|].
+  { by rewrite ba. }
+  move=> cb. apply /orP. right.
+  apply /t_closureP. apply: clos_trans_t1n. apply: t_trans.
+  { apply /clos_t1n_trans /t_closureP. exact: ba. }
+  apply /clos_t1n_trans /t_closureP. exact: cb.
+Qed.
+
+(* Reflexive-transitive closure reflection lemma *)
+Lemma rt_closureP a b :
+  reflect (clos_refl_trans_1n T (sfrel f) a b) (rt_closure a b).
+Proof.
+  apply /(iffP idP).
+  { rewrite /rt_closure. 
+    rewrite in_cons=> /orP[/eqP -> | atb].
+    { constructor. }
+    move: (t_closureP a b). 
+    rewrite /t_closure => refl. move: (refl atb). 
+    elim=> [c d cfd | c d e cfd st rt].
+    { apply: Relation_Operators.rt1n_trans; last by constructor.
+      move: cfd. rewrite /sfrel /filter_neq //=.
+      rewrite mem_filter. by move=> /andP [??]. }
+    apply: Relation_Operators.rt1n_trans; last exact: rt.
+    move: cfd. rewrite /sfrel /filter_neq //=.
+    rewrite mem_filter. move=> /andP [? H]. exact: H. }
+  move=> cab. rewrite /rt_closure /up_set.
+  rewrite in_cons. apply/orP.
+  elim: cab => [| c d e st rt [/eqP -> | efd]]; first by left.
+  { case: (d =P c)=> [eq|neq] //=; first by left.
+    right. move: st. rewrite /sfrel /=.
+    rewrite /s_up_set /Subterm.FixWf Fix_eq; last by apply: ext_s_up_set.
+    rewrite {1}/s_up_set_functional mem_cat /filter_neq mem_filter => ->.
+     apply /orP. left. by apply /predD1P. }
+  case: (d =P c)=> [<-|neq] //=; first by right. 
+  right. move: (t_closureP d e)=> refl. move: (refl efd)=> ct.
+  apply /(t_closureP c e) /clos_trans_t1n /t_trans; first last.
+  { apply: clos_t1n_trans. exact: ct. }
+  apply: t_step. rewrite /sfrel /filter_neq //=. 
+  rewrite mem_filter. by apply /predD1P. 
+Qed.
 
 End well_founded.
